src/typechecker/FStarC.TypeChecker.TermEqAndSimplify.fst
@@ -188,13 +188,13 @@ let rec eq_tm (env:env_t) (t1:term) (t2:term) : ML eq_result =
     | Tm_uvar (u1, ([], _)), Tm_uvar (u2, ([], _)) ->
       equal_if (Unionfind.equiv u1.ctx_uvar_head u2.ctx_uvar_head)
 
-    | Tm_app {hd=h1; args=args1}, Tm_app {hd=h2; args=args2} ->
+    | Tm_app {hd=h1; arg=arg1}, Tm_app {hd=h2; arg=arg2} ->
       begin match (un_uinst h1).n, (un_uinst h2).n with
       | Tm_fvar f1, Tm_fvar f2 when fv_eq f1 f2 && List.mem (string_of_lid (lid_of_fv f1)) injectives ->
-        equal_data f1 args1 f2 args2 0
+        equal_data f1 [arg1] f2 [arg2] 0
 
       | _ -> // can only assert they're equal if they syntactically match, nothing else
-        eq_and (eq_tm env h1 h2) (fun () -> eq_args env args1 args2)
+        eq_and (eq_tm env h1 h2) (fun () -> eq_args env [arg1] [arg2])
       end
 
     | Tm_match {scrutinee=t1; brs=bs1}, Tm_match {scrutinee=t2; brs=bs2} ->  //AR: note: no return annotations
@@ -223,17 +223,13 @@ let rec eq_tm (env:env_t) (t1:term) (t2:term) : ML eq_result =
        * AR: ignoring residual comp here, that's an ascription added by the typechecker
        *     do we care if that's different?
        *)
-    | Tm_abs {bs=bs1; body=body1}, Tm_abs {bs=bs2; body=body2}
-      when List.length bs1 = List.length bs2 ->
+    | Tm_abs {b=b1; body=body1}, Tm_abs {b=b2; body=body2} ->
 
-      eq_and (List.fold_left2 (fun r b1 b2 -> eq_and r (fun () -> eq_tm env b1.binder_bv.sort b2.binder_bv.sort))
-                Equal bs1 bs2)
+      eq_and (eq_tm env b1.binder_bv.sort b2.binder_bv.sort)
              (fun () -> eq_tm env body1 body2)
 
-    | Tm_arrow {bs=bs1; comp=c1}, Tm_arrow {bs=bs2; comp=c2}
-          when List.length bs1 = List.length bs2 ->
-      eq_and (List.fold_left2 (fun r b1 b2 -> eq_and r (fun () -> eq_tm env b1.binder_bv.sort b2.binder_bv.sort))
-                Equal bs1 bs2)
+    | Tm_arrow {b=b1; comp=c1}, Tm_arrow {b=b2; comp=c2} ->
+      eq_and (eq_tm env b1.binder_bv.sort b2.binder_bv.sort)
              (fun () -> eq_comp env c1 c2)
 
     | _ -> Unknown
@@ -448,7 +444,7 @@ let simplify (debug:bool) (env:env_t) (tm:term) : ML term =
              (* Simplify ∀x. True to True *)
              | [(t, _)] ->
                begin match (SS.compress t).n with
-                     | Tm_abs {bs=[_]; body} ->
+                     | Tm_abs {b=_; body} ->
                        (match simp_t body with
                        | Some true -> w U.t_true
                        | _ -> tm)
@@ -457,7 +453,7 @@ let simplify (debug:bool) (env:env_t) (tm:term) : ML term =
              (* Simplify ∀x. True to True, and ∀x. False to False, if the domain is not empty *)
              | [(ty, Some ({ aqual_implicit = true })); (t, _)] ->
                begin match (SS.compress t).n with
-                     | Tm_abs {bs=[_]; body} ->
+                     | Tm_abs {b=_; body} ->
                        (match simp_t body with
                        | Some true -> w U.t_true
                        | Some false when clearly_inhabited ty -> w U.t_false
@@ -470,7 +466,7 @@ let simplify (debug:bool) (env:env_t) (tm:term) : ML term =
              (* Simplify ∃x. False to False *)
              | [(t, _)] ->
                begin match (SS.compress t).n with
-                     | Tm_abs {bs=[_]; body} ->
+                     | Tm_abs {b=_; body} ->
                        (match simp_t body with
                        | Some false -> w U.t_false
                        | _ -> tm)
@@ -479,7 +475,7 @@ let simplify (debug:bool) (env:env_t) (tm:term) : ML term =
              (* Simplify ∃x. False to False and ∃x. True to True, if the domain is not empty *)
              | [(ty, Some ({ aqual_implicit = true })); (t, _)] ->
                begin match (SS.compress t).n with
-                     | Tm_abs {bs=[_]; body} ->
+                     | Tm_abs {b=_; body} ->
                        (match simp_t body with
                        | Some false -> w U.t_false
                        | Some true when clearly_inhabited ty -> w U.t_true
